Add pack and unpack methods, which resolve to peekArray and pokeArray

ffi/ByteStringFFI.v
@@ -53,6 +53,40 @@ Hint Unfold bind.
 Hint Unfold Bind2.
 Hint Unfold allocate_buffer.
 Hint Unfold HeapState.find_free_block.
+Hint Unfold ByteStringHeap.buffer_pack_obligation_1.
+Hint Unfold buffer_pack.
+
+Definition packDSL h xs:
+  reflect_ADT_DSL_computation HeapSpec (buffer_pack xs h).
+Proof.
+  Local Opaque alloc.
+  Local Opaque write.
+  Time compile_term.
+    admit.
+  Local Transparent alloc.
+  Local Transparent write.
+Admitted.
+
+Corollary packDSL_correct : forall (h : Rep HeapSpec) xs,
+  refine (buffer_pack xs h)
+         (denote HeapSpec (projT1 (packDSL h xs))).
+Proof. intros; apply denote_refineEquiv. Qed.
+
+Hint Unfold buffer_unpack.
+
+Definition unpackDSL h bs:
+  reflect_ADT_DSL_computation HeapSpec (buffer_unpack bs h).
+Proof.
+  Local Opaque read.
+  Time compile_term.
+  Local Transparent read.
+Defined.
+
+Corollary unpackDSL_correct : forall (h : Rep HeapSpec) bs,
+  refine (buffer_unpack bs h)
+         (denote HeapSpec (projT1 (unpackDSL h bs))).
+Proof. intros; apply denote_refineEquiv. Qed.
+
 Hint Unfold make_room_by_growing_buffer.
 Hint Unfold make_room_by_shifting_up.
 Hint Unfold ByteStringHeap.buffer_cons_obligation_2.
@@ -145,6 +179,9 @@ Axiom joinIO   : forall {a : Type}, IO (IO a) -> IO a.
 Axiom bindIO_returnIO : forall {a b : Type} (f : a -> b) (x : IO a),
   bindIO x (fun a => returnIO (f a)) = fmapIO f x.
 
+Axiom fmapIO_id : forall {a : Type} (x : IO a),
+  fmapIO id x = x.
+
 Axiom unsafeDupablePerformIO : forall {a : Type}, IO a -> a.
 Axiom unsafeDupablePerformIO_inj : forall {a : Type} x y,
   x = y -> @unsafeDupablePerformIO a x = unsafeDupablePerformIO y.
@@ -159,6 +196,8 @@ Axiom peek    : Ptr Word -> IO Word.
 Axiom poke    : Ptr Word -> Word -> IO ().
 Axiom memcpy  : Ptr Word -> Ptr Word -> Size -> IO ().
 Axiom memset  : Ptr Word -> Size -> Word -> IO ().
+Axiom read    : Ptr Word -> Size -> IO (list Word).
+Axiom write   : Ptr Word -> list Word -> IO ().
 
 Definition ghcDenote {A : Type} : ClientDSL (getADTSig HeapSpec) (Rep HeapSpec) (IO A) -> IO A.
 Proof.
@@ -193,6 +232,12 @@ Proof.
   exact (bindIO (memset (hlist_head (hlist_tail h))
                         (hlist_head (hlist_tail (hlist_tail h)))
                         (hlist_head (hlist_tail (hlist_tail (hlist_tail h)))))
+                (fun _ => y (hlist_head h))).
+  exact (bindIO (read (hlist_head (hlist_tail h))
+                      (hlist_head (hlist_tail (hlist_tail h))))
+                (y (hlist_head h))).
+  exact (bindIO (write (hlist_head (hlist_tail h))
+                      (hlist_head (hlist_tail (hlist_tail h))))
                 (fun _ => y (hlist_head h))).
 Defined.
 
@@ -247,6 +292,54 @@ Defined.
 
 Definition ghcEmptyDSL' := Eval simpl in projT1 ghcEmptyDSL.
 Print ghcEmptyDSL'.
+
+Lemma ghcPackDSL :
+  { f : list Word -> PS
+  & forall r xs,
+      f xs = unsafeDupablePerformIO
+               (ghcDenote ((returnIO \o fst) <$> projT1 (packDSL r xs))) }.
+Proof.
+  eexists; intros.
+  symmetry.
+  simpl projT1.
+  unfold comp.
+(*
+  rewrite !fmap_If.
+  etransitivity.
+    do 3 setoid_rewrite ghcDenote_If.
+    reflexivity.
+  simpl.
+  do 4 (unfold compose, comp; simpl).
+  unfold ghcDenote; simpl.
+  rewrite !bindIO_returnIO.
+  unfold If_Then_Else.
+  higher_order_reflexivity.
+Defined.
+*)
+Admitted.
+
+Definition ghcPackDSL' := Eval simpl in projT1 ghcPackDSL.
+Print ghcPackDSL'.
+
+Lemma ghcUnpackDSL :
+  { f : PS -> list Word
+  & forall r bs,
+      f bs = unsafeDupablePerformIO
+               (ghcDenote (returnIO <$> projT1 (unpackDSL r bs))) }.
+Proof.
+  eexists; intros.
+  symmetry.
+  simpl projT1.
+  unfold comp.
+  simpl.
+  do 4 (unfold compose, comp; simpl).
+  unfold ghcDenote; simpl.
+  rewrite !bindIO_returnIO, fmapIO_id.
+  higher_order_reflexivity.
+Defined.
+
+Definition ghcUnpackDSL' := Eval simpl in projT1 ghcUnpackDSL.
+Print ghcUnpackDSL'.
 
 Lemma ghcConsDSL :
   { f : PS -> Word -> PS
